Revised examples along with the specialization concept

examples/ProcDec.v
@@ -1,6 +1,6 @@
 Require Import Bool String List.
 Require Import Lib.CommonTactics Lib.ilist Lib.Word Lib.Struct Lib.StringBound.
-Require Import Lts.Syntax Lts.Semantics.
+Require Import Lts.Syntax Lts.Semantics Lts.Renaming.
 Require Import Ex.SC Ex.Fifo Ex.MemAtomic.
 
 Set Implicit Arguments.
@@ -11,7 +11,6 @@ Set Implicit Arguments.
  * until getting a memory operation response.
  *)
 Section ProcDec.
-  Variable i: nat.
   Variable inName outName: string.
   Variables addrSize valSize rfIdx: nat.
 
@@ -25,91 +24,90 @@ Section ProcDec.
   Definition opSt : ConstT (Bit 2) := WO~0~1.
   Definition opHt : ConstT (Bit 2) := WO~1~0.
 
-  Notation "^ s" := (s __ i) (at level 0).
-
   (* Called method signatures *)
   Definition memReq := MethodSig (inName -n- "enq")(memAtomK addrSize valSize) : Void.
   Definition memRep := MethodSig (outName -n- "deq")() : memAtomK addrSize valSize.
-  Definition halt := MethodSig ^"HALT"() : Void.
+  Definition halt := MethodSig "HALT"() : Void.
 
   Definition nextPc {ty} ppc st : ActionT ty Void := (
-    Write ^"pc" <- #(getNextPc _ ppc st (dec _ st ppc));
+    Write "pc" <- #(getNextPc _ ppc st (dec _ st ppc));
     Retv
   )%kami.
 
   Definition reqLd {ty} : ActionT ty Void :=
-    (Read stall <- ^"stall";
+    (Read stall <- "stall";
      Assert !#stall;
-     Read ppc <- ^"pc";
-     Read st <- ^"rf";
+     Read ppc <- "pc";
+     Read st <- "rf";
      Assert #(dec _ st ppc)@."opcode" == $$opLd;
      Call memReq(STRUCT {  "type" ::= $$memLd;
                            "addr" ::= #(dec _ st ppc)@."addr";
                            "value" ::= $$Default });
-     Write ^"stall" <- $$true;
+     Write "stall" <- $$true;
      Retv)%kami.
 
   Definition reqSt {ty} : ActionT ty Void :=
-    (Read stall <- ^"stall";
+    (Read stall <- "stall";
      Assert !#stall;
-     Read ppc <- ^"pc";
-     Read st <- ^"rf";
+     Read ppc <- "pc";
+     Read st <- "rf";
      Assert #(dec _ st ppc)@."opcode" == $$opSt;
      Call memReq(STRUCT {  "type" ::= $$opSt;
                            "addr" ::= #(dec _ st ppc)@."addr";
                            "value" ::= #(dec _ st ppc)@."value" });
-     Write ^"stall" <- $$true;
+     Write "stall" <- $$true;
      Retv)%kami.
 
   Definition repLd {ty} : ActionT ty Void :=
     (Call val <- memRep();
-     Read ppc <- ^"pc";
-     Read st <- ^"rf";
+     Read ppc <- "pc";
+     Read st <- "rf";
      Assert #val@."type" == $$opLd;
-     Write ^"rf" <- #st@[#(dec _ st ppc)@."reg" <- #val@."value"];
-     Write ^"stall" <- $$false;
+     Write "rf" <- #st@[#(dec _ st ppc)@."reg" <- #val@."value"];
+     Write "stall" <- $$false;
      nextPc ppc st)%kami.
 
   Definition repSt {ty} : ActionT ty Void :=
     (Call val <- memRep();
-     Read ppc <- ^"pc";
-     Read st <- ^"rf";
+     Read ppc <- "pc";
+     Read st <- "rf";
      Assert #val@."type" == $$opSt;
-     Write ^"stall" <- $$false;
+     Write "stall" <- $$false;
      nextPc ppc st)%kami.
 
   Definition execHt {ty} : ActionT ty Void :=
-    (Read stall <- ^"stall";
+    (Read stall <- "stall";
      Assert !#stall;
-     Read ppc <- ^"pc";
-     Read st <- ^"rf";
+     Read ppc <- "pc";
+     Read st <- "rf";
      Assert #(dec _ st ppc)@."opcode" == $$opHt;
      Call halt();
      Retv)%kami.
 
   Definition execNm {ty} : ActionT ty Void :=
-    (Read stall <- ^"stall";
+    (Read stall <- "stall";
      Assert !#stall;
-     Read ppc <- ^"pc";
-     Read st <- ^"rf";
+     Read ppc <- "pc";
+     Read st <- "rf";
      Assert !(#(dec _ st ppc)@."opcode" == $$opLd
            || #(dec _ st ppc)@."opcode" == $$opSt
            || #(dec _ st ppc)@."opcode" == $$opHt);
-     Write ^"rf" <- #(getNextState _ ppc st);
+     Write "rf" <- #(getNextState _ ppc st);
      nextPc ppc st)%kami.
 
   Definition procDec := MODULE {
-    Register ^"pc" : Bit addrSize <- Default
-    with Register ^"rf" : Vector (Bit valSize) rfIdx <- Default
-    with Register ^"stall" : Bool <- false
+    Register "pc" : Bit addrSize <- Default
+    with Register "rf" : Vector (Bit valSize) rfIdx <- Default
+    with Register "stall" : Bool <- false
 
-    with Rule ^"reqLd" := reqLd
-    with Rule ^"reqSt" := reqSt
-    with Rule ^"repLd" := repLd
-    with Rule ^"repSt" := repSt
-    with Rule ^"execHt" := execHt
-    with Rule ^"execNm" := execNm
+    with Rule "reqLd" := reqLd
+    with Rule "reqSt" := reqSt
+    with Rule "repLd" := repLd
+    with Rule "repSt" := repSt
+    with Rule "execHt" := execHt
+    with Rule "execNm" := execNm
   }.
+
 End ProcDec.
 
 Hint Unfold getNextPc nextPc memReq memRep halt.
@@ -121,10 +119,11 @@ Section ProcDecM.
   Variable dec: DecT 2 addrSize valSize rfIdx.
   Variable exec: ExecT 2 addrSize valSize rfIdx.
 
-  Definition pdeci (i: nat) :=
-    procDec i ("Ins"__ i) ("Outs"__ i) dec exec.
+  Definition pdec := procDec "Ins"%string "Outs"%string dec exec.
 
-  Definition pdecfi (i: nat) := ConcatMod (pdeci i) (iomi addrSize fifoSize (Bit valSize) i).
+  Definition pdecf := ConcatMod pdec (iom addrSize fifoSize (Bit valSize)).
+
+  Definition pdecfi (i: nat) := specializeMod pdecf i.
 
   Fixpoint pdecfs (i: nat) :=
     match i with
@@ -134,21 +133,7 @@ Section ProcDecM.
 
   Definition procDecM (n: nat) := ConcatMod (pdecfs n) (minst addrSize (Bit valSize) n).
 
-  (* Section Facts. *)
-
-  (*   Lemma regsInDomain_pdeci i: RegsInDomain (pdeci i). *)
-  (*   Proof. *)
-  (*     regsInDomain_tac. *)
-  (*   Qed. *)
-
-  (*   Lemma regsInDomain_pdecfi i: RegsInDomain (pdecfi i). *)
-  (*   Proof. *)
-  (*     apply concatMod_RegsInDomain; *)
-  (*     [apply regsInDomain_pdeci|apply regsInDomain_iomi]. *)
-  (*   Qed. *)
-
-  (* End Facts. *)
-
 End ProcDecM.
 
-Hint Unfold pdeci pdecfi pdecfs procDecM : ModuleDefs.
+Hint Unfold pdec pdecf pdecfi pdecfs procDecM : ModuleDefs.
+
