examples/MemAtomic.v
@@ -1,21 +1,18 @@
 Require Import Bool String List.
 Require Import Lib.CommonTactics Lib.ilist Lib.Word Lib.Struct Lib.StringBound.
-Require Import Lts.Syntax Lts.Semantics.
+Require Import Lts.Syntax Lts.Semantics Lts.Renaming.
 Require Import Ex.SC Ex.Fifo.
 
 Set Implicit Arguments.
 
 Section Middleman.
   Variable inName outName: string.
-  Variable memi i: nat.
   Variable addrSize: nat.
   Variable dType: Kind.
 
-  Notation "^ s" := (s __ i) (at level 0).
-
   Definition getReq := MethodSig (inName -n- "deq")() : atomK addrSize dType.
   Definition setRep := MethodSig (outName -n- "enq")(atomK addrSize dType) : Void.
-  Definition exec := MethodSig ("exec"__ memi)(atomK addrSize dType) : atomK addrSize dType.
+  Definition exec := MethodSig "exec"(atomK addrSize dType) : atomK addrSize dType.
 
   Definition processLd {ty} : ActionT ty Void :=
     (Call req <- getReq();
@@ -34,16 +31,9 @@ Section Middleman.
      Retv)%kami.
 
   Definition mid := MODULE {
-    Rule ^"processLd" := processLd
-    with Rule ^"processSt" := processSt
+    Rule "processLd" := processLd
+    with Rule "processSt" := processSt
   }.
-
-  (* Section Facts. *)
-  (*   Lemma regsInDomain_mid: RegsInDomain mid. *)
-  (*   Proof. *)
-  (*     regsInDomain_tac. *)
-  (*   Qed. *)
-  (* End Facts. *)
 
 End Middleman.
 
@@ -58,12 +48,14 @@ Section MemAtomic.
 
   Definition minst := memInst n addrSize dType.
 
-  Definition insi (i: nat) := simpleFifo ("Ins"__ i) fifoSize (atomK addrSize dType).
-  Definition outsi (i: nat) := simpleFifo ("Outs"__ i) fifoSize (atomK addrSize dType).
-  Definition ioi (i: nat) := ConcatMod (insi i) (outsi i).
+  Definition inQ := simpleFifo "Ins" fifoSize (atomK addrSize dType).
+  Definition outQ := simpleFifo "Outs" fifoSize (atomK addrSize dType).
+  Definition ioQ := ConcatMod inQ outQ.
 
-  Definition midi (i: nat) := mid ("Ins"__ i) ("Outs"__ i) i i addrSize dType.
-  Definition iomi (i: nat) := ConcatMod (ioi i) (midi i).
+  Definition midQ := mid "Ins" "Outs" addrSize dType.
+  Definition iom := ConcatMod ioQ midQ.
+
+  Definition iomi (i: nat) := specializeMod iom i.
 
   Fixpoint ioms (i: nat) :=
     match i with
@@ -73,20 +65,7 @@ Section MemAtomic.
 
   Definition memAtomic := ConcatMod (ioms n) minst.
 
-  (* Section Facts. *)
-  (*   Lemma regsInDomain_ioi i: RegsInDomain (ioi i). *)
-  (*   Proof. *)
-  (*     apply concatMod_RegsInDomain; apply regsInDomain_simpleFifo. *)
-  (*   Qed. *)
-
-  (*   Lemma regsInDomain_iomi i: RegsInDomain (iomi i). *)
-  (*   Proof. *)
-  (*     apply concatMod_RegsInDomain; *)
-  (*     [apply regsInDomain_ioi|apply regsInDomain_mid]. *)
-  (*   Qed. *)
-
-  (* End Facts. *)
-
 End MemAtomic.
 
-Hint Unfold minst insi outsi ioi midi iomi ioms memAtomic : ModuleDefs.
+Hint Unfold minst inQ outQ ioQ midQ iom iomi ioms memAtomic : ModuleDefs.
+
